Test/VProg.v
@@ -1,0 +1,123 @@
+Require Import SLFun.Util SLFun.Values SLFun.SL.
+Require Import SLFun.VProg.
+Require SLFun.ConcreteProg SLFun.SLProg.
+
+Require Import Coq.Lists.List.
+
+Module CP := SLFun.ConcreteProg.
+Module SP := SLFun.SLProg.
+
+Import SLNotations.
+Import ListNotations.
+
+
+Definition f_main : fid := 0.
+
+Definition sig_main := mk_f_sig (ptr * ptr) unit.
+
+Definition SIG : sig_context :=
+  fun f => match f with
+  | 0 => Some sig_main
+  | _ => None
+  end.
+
+Definition spec_main_n (ps : ptr * ptr) : SP.Spec.t unit :=
+  let (p0, p1) := ps in {|
+  SP.Spec.pre  := SLprop.ex nat (fun n0 => SLprop.cell p0 n0) **
+                  SLprop.ex nat (fun n1 => SLprop.cell p1 n1);
+  SP.Spec.post := fun _ => SLprop.True;
+|}.
+
+Definition spec_main : SP.f_spec sig_main :=
+  fun ps s => eq s (spec_main_n ps).
+
+Definition SPEC : CP.spec_context SIG :=
+  fun f => match f with
+  | 0 => SP.tr_f_spec spec_main
+  | _ => tt
+  end.
+
+Definition data42 : nat := 42.
+
+Definition vprog_main (ps : ptr * ptr) : instr SPEC unit :=
+  let (p0, p1) := ps in
+  Bind _ (Read  _ p0) (fun v0 =>
+  Bind _ (Write _ p1 data42) (fun _ =>
+  Assert _ [_] (fun '(v1,_) => ([CTX.mka (SLprop.cell p0,  v1)], v1 = v0)))).
+
+Definition impl_main (ps : ptr * ptr) :
+  { i : CP.instr unit | i = i_impl (vprog_main ps) }.
+Proof.
+  unfold i_impl, vprog_main; simpl.
+  case ps as (p, p0); simpl.
+  eexists. reflexivity.
+Defined.
+
+Lemma reduce_spec_t [A ctx] [P : i_spec_t A ctx -> Prop] [s0 s1]
+  (H : P s0)
+  (E : s0 = s1):
+  P s1.
+Proof.
+  rewrite <- E; exact H.
+Qed.
+
+Lemma sls_main (ps : ptr * ptr):
+  SP.sls SPEC (proj1_sig (impl_main ps)) (spec_main_n ps).
+Proof.
+  case impl_main as [? ->]; simpl.
+  case ps as (p0, p1).
+  unfold spec_main_n; SP.normalize.
+  apply SP.ExistsE; intro v0.
+  apply SP.ExistsE; intro v1.
+  eapply SP.Cons.
+  - eapply (proj2_sig (i_spec (vprog_main _) [CTX.mka (SLprop.cell p0, v0); CTX.mka (SLprop.cell p1, v1)]))
+      with (post := fun _ => True).
+    + eapply reduce_spec_t. hnf.
+      unshelve refine (@Bind_SpecI _ _ _ _ _ _ _ _ _ _ _ _ _). 3,4:shelve.
+      1:eexists. 2-5:cbn.
+      { eapply reduce_spec_t. hnf.
+        unshelve refine (@Read_SpecI _ _ _ _). 1:shelve.
+        unshelve eexists. 3:cbn.
+        - exact (Vector.cons _ true _ (Vector.cons _ false _ (Vector.nil _))).
+        - cbn; SLprop.normalize; reflexivity.
+        - cbn; reflexivity. }
+
+      cbn.
+      epose (spec_0 := _).
+      intros x sls_0; unshelve eexists; case sls_0 as [].
+      exact (spec_0 x). unfold spec_0; clear spec_0. 2-4:cbn.
+      eapply reduce_spec_t.
+      unshelve refine (@Bind_SpecI _ _ _ _ _ _ _ _ _ _ _ _ _). 3,4:shelve.
+      1:eexists. 2-5:cbn.
+      { eapply reduce_spec_t. hnf.
+        unshelve refine (@Write_SpecI _ _ _ _ _). 1:shelve.
+        unshelve eexists. 3:cbn.
+        - exact (Vector.cons _ false _ (Vector.cons _ true _ (Vector.nil _))).
+        - cbn; SLprop.normalize; reflexivity.
+        - cbn; reflexivity. }
+
+      cbn.
+      epose (spec_1 := ?[spec_1]).
+      intros _u sls_1; unshelve eexists; case sls_1 as [sl_1 []].
+      exact (spec_1 _u sl_1). unfold spec_1; clear spec_1. 2-4:cbn.
+      { eapply reduce_spec_t.
+        unshelve refine (@Assert_SpecI _ _ _ _ _).
+        1:repeat (constructor; [shelve|]); constructor.
+        all:cbn.
+        - unshelve eexists.
+          + exact (Vector.cons _ false _ (Vector.cons _ true _ (Vector.nil _))).
+          + cbn; SLprop.normalize; reflexivity.
+        - cbn; reflexivity. }
+
+      intros ? [? []]; cbn; reflexivity.
+      intros ? [? []]; cbn; reflexivity.
+      unfold _Abbrev.TF.arrow_ext, _Abbrev.TF.arrow_of_fun, sf_rsel; cbn. reflexivity.
+      intros ? []; cbn; reflexivity.
+      intros ? []; cbn; reflexivity.
+      unfold _Abbrev.TF.arrow_ext, _Abbrev.TF.arrow_of_fun, sf_rsel; cbn. reflexivity.
+    + cbn. auto.
+  - unfold sf_post, sf_post_ctx; cbn.
+    split; cbn.
+    + SLprop.normalize. reflexivity.
+    + constructor.
+Qed.
