VProg.v
@@ -1,0 +1,620 @@
+Require Import SLFun.Util SLFun.Values SLFun.SL.
+Require SLFun.ConcreteProg SLFun.SLProg SLFun.FunProg.
+
+Require Import Coq.Lists.List.
+
+Import SLNotations.
+Import ListNotations.
+
+
+Module Vprop.
+  Record t := mk {
+    ty : Type;
+    sl : ty -> SLprop.t;
+  }.
+  Global Arguments mk [ty].
+End Vprop.
+
+Module CTX.
+  Definition atom := {v : Vprop.t & Vprop.ty v}.
+
+  Definition mka [A : Type] (arg : (A -> SLprop.t) * A) : atom :=
+    let (sl, x) := arg in
+    existT Vprop.ty (Vprop.mk sl) x.
+
+  Definition sla (a : atom): SLprop.t :=
+    Vprop.sl (projT1 a) (projT2 a).
+
+  Definition t := list atom.
+
+  Definition sl : t -> SLprop.t :=
+    List.fold_right (fun a => SLprop.star (sla a)) SLprop.emp.
+
+  Definition app : t -> t -> t := @List.app atom.
+
+  Lemma sl_app (c0 c1 : t):
+    SLprop.eq (sl (app c0 c1)) (sl c0 ** sl c1).
+  Proof.
+    induction c0; simpl; SLprop.normalize; [|rewrite IHc0]; reflexivity.
+  Qed.
+
+  Module Sub.
+    Definition t (c : CTX.t) := Vector.t bool (List.length c).
+
+    Fixpoint sub (c : CTX.t) : t c -> CTX.t :=
+      match c with
+      | nil     => fun _ => nil
+      | x :: xs => fun s =>
+          let (hd, tl) := Vector.uncons s in
+          let ys := sub xs tl in
+          if hd then x :: ys else ys
+      end.
+
+    Definition const (c : CTX.t) (v : bool) : t c :=
+      Vector.const v (List.length c).
+  
+    Lemma sub_const_true c:
+      sub c (Sub.const c true) = c.
+    Proof.
+      induction c; simpl; f_equal; auto.
+    Qed.
+    
+    Lemma sub_const_false c:
+      sub c (Sub.const c false) = nil.
+    Proof.
+      induction c; simpl; f_equal; auto.
+    Qed.
+
+    Definition neg [c : CTX.t] : t c -> t c :=
+      Vector.map negb.
+
+    Definition or [c : CTX.t] : t c -> t c -> t c :=
+      Vector.map2 orb.
+    
+    Definition and [c : CTX.t] : t c -> t c -> t c :=
+      Vector.map2 andb.
+
+    Definition minus [c : CTX.t] : t c -> t c -> t c :=
+      Vector.map2 (fun b0 b1 => andb b0 (negb b1)).
+
+    Fixpoint app [c0 c1 : CTX.t] : forall (s0 : t c0) (s1 : t c1), t (c0 ++ c1).
+    Proof.
+      case c0 as [|hd c0].
+      - intros _ s1. exact s1.
+      - intros s0 s1.
+        case s0 as [hd0 tl0] using Vector.caseS'.
+        constructor.
+        + exact hd0.
+        + exact (app c0 c1 tl0 s1).
+    Defined.
+
+    Lemma sub_app [c0 c1] (s0 : t c0) (s1 : t c1):
+      sub (c0 ++ c1) (app s0 s1) = sub c0 s0 ++ sub c1 s1.
+    Proof.
+      induction c0.
+      - reflexivity.
+      - destruct s0 as [[]] using Vector.caseS';
+        simpl; f_equal; apply IHc0.
+    Qed.
+
+    Lemma map_app [c0 c1] (s0 : t c0) (s1 : t c1) f:
+      Vector.map f (app s0 s1) = app (Vector.map f s0) (Vector.map f s1).
+    Proof.
+      induction c0.
+      - reflexivity.
+      - destruct s0 using Vector.caseS'.
+        simpl; f_equal; apply IHc0.
+    Qed.
+
+    Lemma map2_app [c0 c1] (a0 b0 : t c0) (a1 b1 : t c1) f:
+      Vector.map2 f (app a0 a1) (app b0 b1) = app (Vector.map2 f a0 b0) (Vector.map2 f a1 b1).
+    Proof.
+      induction c0.
+      - reflexivity.
+      - destruct a0 using Vector.caseS'.
+        destruct b0 using Vector.caseS'.
+        simpl; f_equal; apply IHc0.
+    Qed.
+
+    Fixpoint split (c0 c1 : CTX.t) : forall (s : t (c0 ++ c1)), t c0 * t c1.
+    Proof.
+      case c0 as [|? c0].
+      - intro s; split. constructor. exact s.
+      - intros [hd tl]%Vector.uncons.
+        case (split c0 c1 tl) as (s0, s1).
+        exact (Vector.cons _ hd _ s0, s1).
+    Defined.
+  
+    Lemma app_split (c0 c1 : CTX.t) (s : Sub.t (c0 ++ c1)):
+      let s01 := Sub.split c0 c1 s in
+      s = Sub.app (fst s01) (snd s01).
+    Proof.
+      induction c0.
+      - reflexivity.
+      - case s as [hd tl] using Vector.caseS'; simpl.
+        specialize (IHc0 tl).
+        destruct Sub.split; simpl in *.
+        rewrite IHc0; reflexivity.
+    Qed.
+
+    Lemma split_app (c0 c1 : CTX.t) (s0 : t c0) (s1 : t c1):
+      split c0 c1 (app s0 s1) = (s0, s1).
+    Proof.
+      induction c0.
+      - destruct s0 using Vector.case0. reflexivity.
+      - destruct s0 as [? s0] using Vector.caseS'; simpl.
+        rewrite (IHc0 s0); reflexivity.
+    Qed.
+
+
+    Fixpoint push [c : CTX.t] : forall (s0 : t c), t c -> t (sub c s0).
+    Proof.
+      case c as [|c0 c].
+      - intros ? _; apply Vector.nil.
+      - intro s0.
+        case s0 as [hd0 tl0] using Vector.caseS'.
+        intros [hd1 tl1]%Vector.uncons.
+        pose (tl2 := @push c tl0 tl1).
+        case hd0; simpl.
+        + exact (Vector.cons _ hd1 _ tl2).
+        + exact tl2.
+    Defined.
+
+    Lemma push_map [c] (s0 s1 : t c) f:
+      push s0 (Vector.map f s1) = Vector.map f (push s0 s1).
+    Proof.
+      induction c; simpl.
+      - reflexivity.
+      - destruct s0 as [h ?] using Vector.caseS'; destruct s1 using Vector.caseS'; simpl.
+        rewrite IHc.
+        case h; reflexivity.
+    Qed.
+
+    Lemma sub_push [c] (s0 s1 : t c):
+      sub (sub c s0) (push s0 s1) = sub c (and s0 s1).
+    Proof.
+      induction c; simpl.
+      - reflexivity.
+      - destruct s0 as [h0 ?] using Vector.caseS'; destruct s1 using Vector.caseS'; simpl.
+        case h0; simpl; rewrite IHc; reflexivity.
+    Qed.
+    
+    Fixpoint pull [c : CTX.t] : forall (s0 : t c), t (sub c s0) -> t (sub c (neg s0)) -> t c.
+    Proof.
+      case c as [|c0 c].
+      - intros ? _ _; apply Vector.nil.
+      - intro s0.
+        case s0 as [hd0 tl0] using Vector.caseS'.
+        case hd0; simpl.
+        + intros [hd1 tl1]%Vector.uncons s2.
+          exact (Vector.cons _ hd1 _ (pull c tl0 tl1 s2)).
+        + intros s1 [hd2 tl2]%Vector.uncons.
+          exact (Vector.cons _ hd2 _ (pull c tl0 s1 tl2)).
+    Defined.
+
+    Lemma map_pull c s0 s1 s2 f:
+      Vector.map f (@pull c s0 s1 s2) = pull s0 (Vector.map f s1) (Vector.map f s2).
+    Proof.
+      induction c as [|c0 c].
+      - reflexivity.
+      - case s0 as [[] s0] using Vector.caseS'.
+        + case s1 as [] using Vector.caseS'; simpl; f_equal; apply IHc.
+        + case s2 as [] using Vector.caseS'; simpl; f_equal; apply IHc.
+    Qed.
+
+    Lemma sl_pull c s0 s1 s2:
+      SLprop.eq (sl (sub c (pull s0 s1 s2)))
+                (sl (sub (sub c s0) s1) ** sl (sub (sub c (neg s0)) s2)).
+    Proof.
+      induction c as [|c0 c].
+      - simpl; SLprop.normalize; reflexivity.
+      - case s0 as [[] s0] using Vector.caseS'.
+        + case s1 as [[]] using Vector.caseS'; simpl;
+            rewrite IHc; SLprop.normalize; reflexivity.
+        + case s2 as [[]] using Vector.caseS'; simpl;
+            rewrite IHc; SLprop.normalize; [rewrite SLprop.star_comm12|]; reflexivity.
+    Qed.
+  End Sub.
+
+  Definition sub : forall c : t, Sub.t c -> t := Sub.sub.
+
+  Lemma sl_split (c : t) (s : Sub.t c):
+    SLprop.eq (sl c) (sl (sub c s) ** sl (sub c (Sub.neg s))).
+  Proof.
+    induction c; simpl.
+    - SLprop.normalize; reflexivity.
+    - case s as [hd tl] using Vector.caseS'; simpl.
+      rewrite (IHc tl).
+      case hd; simpl; SLprop.normalize.
+      + reflexivity.
+      + apply SLprop.star_comm12.
+  Qed.
+
+  Module Inj.
+    Local Set Implicit Arguments.
+
+    Record t (c0 c1 : CTX.t) := {
+      img : Sub.t c1;
+      ieq : SLprop.eq (sl (sub c1 img)) (sl c0);
+    }.
+  End Inj.
+End CTX.
+
+Module VpropList.
+  Definition t := list Vprop.t.
+
+  Definition sel : t -> list Type := map Vprop.ty.
+  Definition sel_t (vs : t) := Tuple.t (sel vs).
+
+  Fixpoint inst (vs : t) {struct vs} : sel_t vs -> CTX.t :=
+    match vs with
+    | nil     => fun _ => nil
+    | v :: vs => fun '(sel, sels) => existT _ v sel :: inst vs sels
+    end.
+
+  Definition of_ctx : CTX.t -> t :=
+    map (@projT1 _ _).
+
+  Fixpoint sel_of_ctx (c : CTX.t) : sel_t (of_ctx c) :=
+    match c with
+    | nil => tt
+    | existT _ v s :: c => (s, sel_of_ctx c)
+    end.
+
+  Lemma inst_of_ctx ctx:
+    inst (of_ctx ctx) (sel_of_ctx ctx) = ctx.
+  Proof.
+    induction ctx as [|[]]; simpl; f_equal; auto.
+  Qed.
+
+  Fixpoint app_sel [vs0 vs1 : t] (ss0 : sel_t vs0) (ss1 : sel_t vs1) : sel_t (vs0 ++ vs1) :=
+    match vs0 as vs0 return sel_t vs0 -> sel_t (vs0 ++ vs1) with
+    | nil       => fun _ => ss1
+    | v0 :: vs0 => fun '(s0, ss0) => (s0, app_sel ss0 ss1)
+    end ss0.
+  
+  Lemma inst_app vs0 vs1 ss0 ss1:
+    inst (vs0 ++ vs1) (app_sel ss0 ss1) = inst vs0 ss0 ++ inst vs1 ss1.
+  Proof.
+    induction vs0; simpl.
+    - reflexivity.
+    - case ss0 as (s0, ss0); simpl.
+      rewrite IHvs0; reflexivity.
+  Qed.
+End VpropList.
+
+Module _Abbrev.
+  Module CP  := SLFun.ConcreteProg.
+  Module SP  := SLFun.SLProg.
+  Module FP  := SLFun.FunProg.
+  Module TF  := FP.TF.
+  Module Sub := CTX.Sub.
+End _Abbrev.
+Import _Abbrev.
+
+Section VProg.
+  Context [SIG : sig_context] (SPC : CP.spec_context SIG).
+
+(* [instr] *)
+
+Local Set Implicit Arguments.
+Record i_spec_t (A : Type) (ctx : CTX.t) := mk_i_spec {
+  sf_csm  : Sub.t ctx;
+  sf_prd  : A -> VpropList.t;
+  sf_spec : FP.instr (FP.TF.mk_p A (fun x => VpropList.sel (sf_prd x)));
+}.
+Local Unset Implicit Arguments.
+
+Definition sf_rsel [A ctx] (s : i_spec_t A ctx) (x : A) : list Type :=
+  VpropList.sel (sf_prd s x).
+Definition sf_rvar [A ctx] (s : i_spec_t A ctx) : TF.p :=
+  TF.mk_p A (sf_rsel s).
+
+Definition sf_post_ctx [A ctx] (s : i_spec_t A ctx) (x : A) (sels : VpropList.sel_t (sf_prd s x)) : CTX.t :=
+  VpropList.inst (sf_prd s x) sels ++ CTX.sub ctx (Sub.neg (sf_csm s)).
+
+Definition sf_post [A ctx] (s : i_spec_t A ctx) (post : TF.t (sf_rvar s) -> Prop) (x : A) : SLprop.t :=
+  SLprop.ex (VpropList.sel_t (sf_prd s x)) (fun sels =>
+    SLprop.pure (post (TF.mk (sf_rsel s) x sels)) **
+    CTX.sl (sf_post_ctx s x sels))%slprop.
+
+Definition sound_spec [A : Type] (i : @CP.instr SIG A) (ctx : CTX.t) (s : i_spec_t A ctx) : Prop :=
+  forall (post : TF.t (sf_rvar s) -> Prop)
+         (PRE : FP.wlp (sf_spec s) post),
+  SP.sls SPC i {|
+    SP.Spec.pre  := CTX.sl ctx;
+    SP.Spec.post := sf_post s post;
+  |}.
+
+Definition i_spec_p [A : Type] (i : @CP.instr SIG A) (ctx : CTX.t) : Type :=
+  { sp : i_spec_t A ctx -> Prop | forall s (SP : sp s), sound_spec i ctx s }.
+
+Local Set Implicit Arguments.
+Record instr (A : Type) := mk_instr {
+  i_impl : @CP.instr SIG A;
+  i_spec : forall ctx : CTX.t, i_spec_p i_impl ctx;
+}.
+Local Unset Implicit Arguments.
+
+(* Transformation *)
+
+Section AddCsm.
+  Context [A : Type] [ctx : CTX.t] (s : i_spec_t A ctx) (csm : Sub.t ctx).
+  
+  Let acsm := CTX.sub ctx (Sub.minus csm (sf_csm s)).
+
+  Definition add_csm : i_spec_t A ctx
+    :=
+    {|
+      sf_csm  := Sub.or (sf_csm s) csm;
+      sf_prd  := fun x => sf_prd s x ++ VpropList.of_ctx acsm;
+      sf_spec := FP.Bind (sf_spec s) (fun x =>
+                   FP.Ret (TF.mk _ (TF.v_val x) (VpropList.app_sel (TF.v_sel x) (VpropList.sel_of_ctx acsm)))
+                 )
+    |}.
+
+  Lemma add_csm_sound (i : @CP.instr SIG A):
+    sound_spec i ctx s -> sound_spec i ctx add_csm.
+  Proof.
+    intros S0 post PRE; simpl in PRE.
+    eapply SP.Cons.
+    apply S0, PRE.
+    split; simpl. reflexivity.
+    intro x; unfold add_csm, sf_post, sf_post_ctx, sf_rsel; cbn.
+    apply SLprop.imp_exists_l; intro sel0.
+    apply SLprop.imp_exists_r with (wit := VpropList.app_sel sel0 (VpropList.sel_of_ctx acsm)).
+    apply SLprop.star_morph_imp. reflexivity.
+    rewrite VpropList.inst_app, !CTX.sl_app; SLprop.normalize.
+    apply SLprop.star_morph_imp. reflexivity.
+    unfold acsm; rewrite VpropList.inst_of_ctx.
+    set (c0 := CTX.sub ctx (Sub.neg (sf_csm s))).
+    rewrite (CTX.sl_split c0 (Sub.push (Sub.neg (sf_csm s)) csm)).
+    unfold Sub.neg, CTX.sub, c0; rewrite <- Sub.push_map with (f := negb).
+    rewrite !Sub.sub_push.
+    apply R_refl. reflexivity.
+    do 3 f_equal; apply Vector.ext; intro k;
+      unfold Sub.and, Sub.or, Sub.minus;
+      repeat progress (erewrite ?Vector.nth_map2, ?Vector.nth_map by reflexivity).
+    - apply Bool.andb_comm.
+    - symmetry; apply Bool.negb_orb.
+  Qed.
+End AddCsm.
+
+(* Constructors *)
+
+Section Ret.
+  Context [A : Type] (x : A) (sp : A -> list Vprop.t).
+
+  Inductive Ret_Spec (ctx : CTX.t) : i_spec_t A ctx -> Prop
+    := Ret_SpecI
+    (sels : Tuple.t (map Vprop.ty (sp x)))
+    (ij : CTX.Inj.t (VpropList.inst (sp x) sels) ctx) :
+    Ret_Spec ctx {|
+      sf_csm  := CTX.Inj.img ij;
+      sf_prd  := sp;
+      sf_spec := FP.Ret (TF.mk (fun x => VpropList.sel (sp x)) x sels);
+    |}.
+
+  Program Definition Ret : instr A := {|
+    i_impl := CP.Ret x;
+    i_spec := fun ctx => Ret_Spec ctx;
+  |}.
+  Next Obligation.
+    destruct SP; do 2 intro; simpl in *.
+    eapply SP.CFrame with (fr := CTX.sl (CTX.sub ctx (Sub.neg (CTX.Inj.img ij)))).
+    - apply SP.Ret
+       with (sp := fun x' => (SLprop.pure (x' = x) ** CTX.sl (VpropList.inst (sp x) sels))%slprop).
+    - split; simpl.
+      + SLprop.normalize. apply SLprop.imp_pure_r. reflexivity.
+        rewrite CTX.sl_split with (s := CTX.Inj.img ij).
+        apply SLprop.star_morph_imp. 2:reflexivity.
+        rewrite (CTX.Inj.ieq ij); reflexivity.
+      + intro x'. SLprop.normalize. apply SLprop.imp_pure_l. intros ->.
+        unfold sf_post; cbn.
+        apply SLprop.imp_exists_r with (wit := sels).
+        apply SLprop.imp_pure_r. assumption.
+        rewrite CTX.sl_app. reflexivity.
+  Qed.
+End Ret.
+Section Bind.
+  Context [A B : Type] (f : instr A) (g : A -> instr B).
+  
+  Local Opaque TF.arrow_ext.
+
+  Inductive Bind_Spec (ctx : CTX.t) : i_spec_t B ctx -> Prop
+    := Bind_SpecI : forall
+    (s_fp : {s_f : i_spec_t A ctx
+                 | proj1_sig (i_spec f ctx) s_f}),
+    let s_f := proj1_sig s_fp in
+    let f_prd x sels :=
+      Sub.app (Sub.const (VpropList.inst (sf_prd s_f x) sels) true)
+                  (Sub.const (CTX.sub ctx (Sub.neg (sf_csm s_f))) false)
+    in forall
+    (s_gp : forall (x : A) (sels : VpropList.sel_t (sf_prd s_f x)),
+            let ctx1 := sf_post_ctx s_f x sels in
+            {s_g : i_spec_t B ctx1
+                 | proj1_sig (i_spec (g x) ctx1) s_g}),
+    let s_g := fun x sels => add_csm (proj1_sig (s_gp x sels)) (f_prd x sels)
+    in forall
+    (csm : Sub.t ctx)
+    (CSM : forall x sels,
+      Sub.pull (sf_csm s_f) (Sub.const _ true) (snd (Sub.split _ _ (sf_csm (s_g x sels))))
+      = csm)
+    (prd : B -> VpropList.t)
+    (PRD : forall x sels, sf_prd (s_g x sels) = prd),
+    Bind_Spec ctx {|
+      sf_csm  := csm;
+      sf_prd  := prd;
+      sf_spec :=
+          let TF_A     := TF.mk_p A (sf_rsel s_f) in
+          let TF_B prd := TF.mk_p B (fun y => VpropList.sel (prd y)) in
+          @FP.Bind TF_A (TF_B prd)
+              (sf_spec s_f)
+              (TF.arrow_ext TF_A (fun x =>
+                eq_rect _ (fun prd => FP.instr (TF_B prd))
+                          (sf_spec (s_g (TF.v_val x) (TF.v_sel x)))
+                          _ (PRD (TF.v_val x) (TF.v_sel x))))
+    |}.
+  
+  Program Definition Bind : instr B := {|
+    i_impl := CP.Bind (i_impl f) (fun x => i_impl (g x));
+    i_spec := fun ctx => Bind_Spec ctx;
+  |}.
+  Next Obligation.
+    destruct SP; do 2 intro.
+    assert (s_g_sound : forall x sels, sound_spec (i_impl (g x)) _ (s_g x sels)).
+      { intros; apply add_csm_sound, (proj2_sig (i_spec (g x) _) _ (proj2_sig (s_gp x sels))). }
+    assert (s_g_csm : forall x sels, exists csm,
+        sf_csm (s_g x sels) = Sub.app (Sub.const _ true) csm). {
+      intros; exists (snd (Sub.split _ _ (sf_csm (proj1_sig (s_gp x sels))))).
+      unfold s_g, f_prd; simpl; clear.
+      rewrite (Sub.app_split _ _ (sf_csm (proj1_sig (s_gp x sels)))) at 1.
+      unfold Sub.const, Sub.or.
+      etransitivity. apply Sub.map2_app.
+      f_equal; apply Vector.ext; intro k;
+        erewrite Vector.nth_map2, !Vector.const_nth by reflexivity;
+        destruct (Vector.nth _ k); reflexivity.
+    }
+    clearbody s_g; clear s_gp.
+    eapply SP.Bind.
+    - apply (proj2_sig (i_spec f ctx) _ (proj2_sig s_fp)).
+      simpl in PRE; apply PRE.
+    - clear PRE.
+      intro x; unfold sf_post; simpl.
+      apply SP.ExistsE; intro sels0.
+      apply SP.PureE; rewrite TF.arrow_ext_id; simpl; intro PRE.
+      destruct (PRD x sels0); simpl in PRE.
+      eapply SP.Cons.
+        { apply s_g_sound, PRE. }
+      clear PRE.
+      split. reflexivity.
+      intro y; unfold sf_post, sf_post_ctx, sf_rsel; simpl.
+      apply SLprop.imp_exists_l; intro sels1.
+      apply SLprop.imp_pure_l; intro POST.
+      apply SLprop.imp_exists_r with (wit := sels1).
+      apply SLprop.imp_pure_r. exact POST.
+      rewrite <- (CSM x sels0).
+      ecase s_g_csm as [g_csm E]. unfold sf_post_ctx in *; erewrite E.
+      clear.
+      rewrite !CTX.sl_app. apply SLprop.star_morph_imp. reflexivity.
+      rewrite Sub.split_app; simpl.
+      unfold Sub.neg, Sub.const.
+      rewrite Sub.map_app, Sub.sub_app, Sub.map_pull, !Vector.map_const; simpl.
+      rewrite Sub.sl_pull.
+      rewrite !Sub.sub_const_false; simpl; SLprop.normalize; reflexivity.
+  Qed.
+End Bind.
+Section Assert.
+  Context (A : list Type) (P : Tuple.t A -> CTX.t * Prop).
+
+  Inductive Assert_Spec (ctx : CTX.t) : i_spec_t unit ctx -> Prop
+    := Assert_SpecI
+    (p : Tuple.t A)
+    (ij : CTX.Inj.t (fst (P p)) ctx):
+    Assert_Spec ctx {|
+      sf_csm  := Sub.const ctx false;
+      sf_prd  := fun _ => nil;
+      sf_spec := FP.Assert (snd (P p))
+    |}.
+  
+  Program Definition Assert : instr unit := {|
+    i_impl := SP.sl_assert (SLprop.ex (Tuple.t A) (fun p =>
+                SLprop.pure (snd (P p)) ** CTX.sl (fst (P p))))%slprop;
+    i_spec := fun ctx => Assert_Spec ctx;
+  |}.
+  Next Obligation.
+    destruct SP; do 2 intro; simpl in *.
+    case PRE as (PRE & POST).
+    eapply SP.CFrame with (fr := CTX.sl (CTX.sub ctx (Sub.neg (CTX.Inj.img ij)))).
+    - apply SP.Assert_imp with (Q := CTX.sl (fst (P p))).
+      apply SLprop.imp_exists_r with (wit := p).
+      apply SLprop.imp_pure_r. exact PRE.
+      reflexivity.
+    - eenough (SLprop.eq (CTX.sl ctx) _) as sl_eq.
+      split; unfold sf_post, sf_post_ctx, sf_rsel; simpl.
+      + rewrite sl_eq; reflexivity.
+      + intros []; SLprop.normalize.
+        apply SLprop.imp_exists_r with (wit := tt).
+        apply SLprop.imp_pure_r. exact POST.
+        unfold Sub.neg, Sub.const; rewrite Vector.map_const; simpl.
+        rewrite Sub.sub_const_true.
+        rewrite sl_eq; reflexivity.
+      + rewrite CTX.sl_split with (s := CTX.Inj.img ij).
+        setoid_rewrite (CTX.Inj.ieq ij).
+        reflexivity.
+  Qed.
+End Assert.
+Section Read.
+  Context (p : ptr).
+
+  Inductive Read_Spec (ctx : CTX.t) : i_spec_t memdata ctx -> Prop
+    := Read_SpecI
+    (d : memdata)
+    (ij : CTX.Inj.t [CTX.mka (SLprop.cell p, d)] ctx):
+    Read_Spec ctx {|
+      sf_csm  := Sub.const ctx false;
+      sf_prd  := fun _ => nil;
+      sf_spec := FP.Ret (TF.mk (fun _ => nil) d tt);
+    |}.
+
+  Program Definition Read : instr memdata := {|
+    i_impl := CP.Read p;
+    i_spec := fun ctx => Read_Spec ctx;
+  |}.
+  Next Obligation.
+    destruct SP; do 2 intro; simpl in *.
+    eapply SP.CFrame with (fr := CTX.sl (CTX.sub ctx (Sub.neg (CTX.Inj.img ij)))).
+    - eapply SP.Read with (d := d).
+    - eassert (IEq : SLprop.eq _ _). {
+        etransitivity. apply (CTX.Inj.ieq ij).
+        simpl; SLprop.normalize.
+      }
+      split; simpl.
+      + rewrite CTX.sl_split with (s := CTX.Inj.img ij).
+        apply SLprop.star_morph_imp. 2:reflexivity.
+        rewrite IEq; reflexivity.
+      + intro x'. SLprop.normalize. apply SLprop.imp_pure_l. intros ->.
+        unfold sf_post; simpl; SLprop.normalize.
+        apply SLprop.imp_exists_r with (wit := tt).
+        apply SLprop.imp_pure_r. assumption.
+        etransitivity. apply SLprop.star_morph_imp. 2:reflexivity. 
+        eapply SLprop.imp_morph. symmetry in IEq; exact IEq. 1,2:reflexivity.
+        rewrite <- CTX.sl_split.
+        unfold Sub.neg, Sub.const; rewrite Vector.map_const; simpl.
+        rewrite Sub.sub_const_true.
+        reflexivity.
+  Qed.
+End Read.
+Section Write.
+  Context (p : ptr) (d : memdata).
+
+  Inductive Write_Spec (ctx : CTX.t) : i_spec_t unit ctx -> Prop
+    := Write_SpecI
+    (d0 : memdata)
+    (ij : CTX.Inj.t [CTX.mka (SLprop.cell p, d0)] ctx):
+    Write_Spec ctx {|
+      sf_csm  := CTX.Inj.img ij;
+      sf_prd  := fun _ => [Vprop.mk (SLprop.cell p)];
+      sf_spec := FP.Ret (TF.mk (fun _ => [memdata]) tt (d, tt));
+    |}.
+
+  Program Definition Write : instr unit := {|
+    i_impl := CP.Write p d;
+    i_spec := fun ctx => Write_Spec ctx;
+  |}.
+  Next Obligation.
+    destruct SP; do 2 intro; simpl in *.
+    eapply SP.CFrame with (fr := CTX.sl (CTX.sub ctx (Sub.neg (CTX.Inj.img ij)))).
+    - eapply SP.Write with (d0 := d0).
+    - split; unfold sf_post, sf_post_ctx, sf_rsel; simpl.
+      + rewrite CTX.sl_split with (s := CTX.Inj.img ij).
+        apply SLprop.star_morph_imp. 2:reflexivity.
+        rewrite (CTX.Inj.ieq ij); simpl; SLprop.normalize; reflexivity.
+      + intros []; SLprop.normalize.
+        apply SLprop.imp_exists_r with (wit := (d, tt)).
+        apply SLprop.imp_pure_r. assumption.
+        reflexivity.
+  Qed.
+End Write.
+
+End VProg.
